James C - moderate name cleanup (no actual changes)

Assembler.thy
@@ -9,7 +9,7 @@ primrec machine_length :: "assembly \<Rightarrow> nat" where
 
 primrec converted_length :: "assembly list \<Rightarrow> nat" where
   "converted_length [] = 0"
-| "converted_length (a # \<pi>) = machine_length a + converted_length \<pi>"
+| "converted_length (\<iota> # \<pi>) = machine_length \<iota> + converted_length \<pi>"
 
 fun build_symbol_table :: "program \<Rightarrow> symbol \<rightharpoonup> nat" where
   "build_symbol_table [] s = None"
@@ -20,7 +20,7 @@ fun build_symbol_table :: "program \<Rightarrow> symbol \<rightharpoonup> nat" w
 definition get_block_addr :: "(symbol \<rightharpoonup> nat) \<Rightarrow> symbol \<Rightarrow> int" where
   "get_block_addr \<rho> s = int (the (\<rho> s))"
 
-primrec instruction_conv :: "(symbol \<rightharpoonup> nat) \<Rightarrow> assembly \<Rightarrow> instruction list" where
+primrec instruction_conv :: "(symbol \<rightharpoonup> nat) \<Rightarrow> assembly \<Rightarrow> machine_instruction list" where
   "instruction_conv \<rho> (AAssm x) = [AInstr x]"
 | "instruction_conv \<rho> (CAssm dst cmp) = [CInstr dst cmp {}]"
 | "instruction_conv \<rho> (JAssm jmp s) = [AInstr (get_block_addr \<rho> s), CInstr {} (Reg D) jmp]"
@@ -28,7 +28,7 @@ primrec instruction_conv :: "(symbol \<rightharpoonup> nat) \<Rightarrow> assemb
 definition get_assembly :: "program \<Rightarrow> assembly list" where
   "get_assembly \<Pi> = concat (map snd \<Pi>)"
 
-definition program_convert :: "program \<Rightarrow> instruction list" where
+definition program_convert :: "program \<Rightarrow> machine_instruction list" where
   "program_convert \<Pi> = concat (map (instruction_conv (build_symbol_table \<Pi>)) (get_assembly \<Pi>))"
 
 definition get_pc :: "program \<Rightarrow> assembly list \<Rightarrow> nat set" where
@@ -36,8 +36,8 @@ definition get_pc :: "program \<Rightarrow> assembly list \<Rightarrow> nat set"
     { the (build_symbol_table \<Pi> s) + converted_length \<pi>' | s \<pi>'. lookup \<Pi> s = Some (\<pi>' @ \<pi>) }"
 
 fun state_convert :: "program \<Rightarrow> assembly_state \<Rightarrow> machine_state set" where
-  "state_convert \<Pi> (\<sigma>, Some a, d, \<pi>) = {(\<sigma>, a, d, pc) | pc. pc \<in> get_pc \<Pi> \<pi>}"
-| "state_convert \<Pi> (\<sigma>, None, d, \<pi>) = {(\<sigma>, a, d, pc) | a pc. pc \<in> get_pc \<Pi> \<pi>}"
+  "state_convert \<Pi> (\<mu>, Some a, d, \<pi>) = {(\<mu>, a, d, pc) | pc. pc \<in> get_pc \<Pi> \<pi>}"
+| "state_convert \<Pi> (\<mu>, None, d, \<pi>) = {(\<mu>, a, d, pc) | a pc. pc \<in> get_pc \<Pi> \<pi>}"
 
 (* conversion correctness *)
 
@@ -47,15 +47,15 @@ lemma [simp]: "lookup \<Pi> s = Some \<pi> \<Longrightarrow> \<exists>n. build_s
 lemma [simp]: "lookup \<Pi> s = Some \<pi> \<Longrightarrow> nat (get_block_addr (build_symbol_table \<Pi>) s) \<in> get_pc \<Pi> \<pi>" 
   by (induction \<Pi> s rule: lookup.induct) (auto simp add: get_block_addr_def get_pc_def)
 
-lemma instr_conv_len [simp]: "length (instruction_conv \<rho> a) = machine_length a"
-  by (induction a) simp_all
+lemma instr_conv_len [simp]: "length (instruction_conv \<rho> \<iota>) = machine_length \<iota>"
+  by (induction \<iota>) simp_all
 
 lemma convert_expands [simp]: "length \<pi> \<le> converted_length \<pi>"
   proof (induction \<pi>)
   case Nil
     thus ?case by simp
-  case (Cons a \<pi>)
-    thus ?case by (induction a) simp_all
+  case (Cons \<iota> \<pi>)
+    thus ?case by (induction \<iota>) simp_all
   qed
 
 lemma [simp]: "length (concat (map (instruction_conv \<rho>) \<pi>)) = converted_length \<pi>"
@@ -64,14 +64,14 @@ lemma [simp]: "length (concat (map (instruction_conv \<rho>) \<pi>)) = converted
 lemma [simp]: "converted_length (\<pi> @ \<pi>') = converted_length \<pi> + converted_length \<pi>'"
   by (induction \<pi>) simp_all
 
-lemma pc_within: "pc \<in> get_pc \<Pi> (a # \<pi>) \<Longrightarrow> 
-    i < length (instruction_conv (build_symbol_table \<Pi>) a) \<Longrightarrow> i + pc < length (program_convert \<Pi>)"
+lemma pc_within: "pc \<in> get_pc \<Pi> (\<iota> # \<pi>) \<Longrightarrow> 
+    i < length (instruction_conv (build_symbol_table \<Pi>) \<iota>) \<Longrightarrow> i + pc < length (program_convert \<Pi>)"
   proof -
-    assume "pc \<in> get_pc \<Pi> (a # \<pi>)" 
+    assume "pc \<in> get_pc \<Pi> (\<iota> # \<pi>)" 
     then obtain s \<pi>' where P: "pc = the (build_symbol_table \<Pi> s) + converted_length \<pi>'" 
-      and L: "lookup \<Pi> s = Some (\<pi>' @ a # \<pi>)" by (auto simp add: get_pc_def)
-    assume "i < length (instruction_conv (build_symbol_table \<Pi>) a)"
-    hence "i < machine_length a" by simp
+      and L: "lookup \<Pi> s = Some (\<pi>' @ \<iota> # \<pi>)" by (auto simp add: get_pc_def)
+    assume "i < length (instruction_conv (build_symbol_table \<Pi>) \<iota>)"
+    hence "i < machine_length \<iota>" by simp
     with L have "i + the (build_symbol_table \<Pi> s) + converted_length \<pi>' < 
         length (program_convert \<Pi>)"
       proof (induction \<Pi> s rule: build_symbol_table.induct)
@@ -91,24 +91,24 @@ lemma pc_within: "pc \<in> get_pc \<Pi> (a # \<pi>) \<Longrightarrow>
     with P show ?thesis by simp
   qed
 
-lemma [simp]: "pc \<in> get_pc \<Pi> (a # \<pi>) \<Longrightarrow> pc < length (program_convert \<Pi>)"
-  using pc_within by (induction a) fastforce+
+lemma [simp]: "pc \<in> get_pc \<Pi> (\<iota> # \<pi>) \<Longrightarrow> pc < length (program_convert \<Pi>)"
+  using pc_within by (induction \<iota>) fastforce+
 
 lemma [simp]: "pc \<in> get_pc \<Pi> (JAssm jmp s # \<pi>) \<Longrightarrow> Suc pc < length (program_convert \<Pi>)"
   using pc_within by fastforce
 
-lemma [simp]: "i < machine_length a \<Longrightarrow> (instruction_conv \<rho> a @ \<pi>) ! i = instruction_conv \<rho> a ! i"
-  by (induction a) (simp_all, induction i, simp_all)
+lemma [simp]: "i < machine_length \<iota> \<Longrightarrow> (instruction_conv \<rho> \<iota> @ \<pi>) ! i = instruction_conv \<rho> \<iota> ! i"
+  by (induction \<iota>) (simp_all, induction i, simp_all)
 
-lemma lookup_convert': "i < machine_length a \<Longrightarrow> 
-  concat (map (instruction_conv \<rho>) (\<pi> @ a # \<pi>')) ! (converted_length \<pi> + i) = 
-    instruction_conv \<rho> a ! i"
+lemma lookup_convert': "i < machine_length \<iota> \<Longrightarrow> 
+  concat (map (instruction_conv \<rho>) (\<pi> @ \<iota> # \<pi>')) ! (converted_length \<pi> + i) = 
+    instruction_conv \<rho> \<iota> ! i"
   proof (induction \<pi>)
   case Nil
     thus ?case by simp
-  next case (Cons a' \<pi>)
-    hence "(instruction_conv \<rho> a' @ concat (map (instruction_conv \<rho>) (\<pi> @ a # \<pi>'))) ! 
-        (length (instruction_conv \<rho> a') + converted_length \<pi> + i) = instruction_conv \<rho> a ! i" 
+  next case (Cons \<iota>' \<pi>)
+    hence "(instruction_conv \<rho> \<iota>' @ concat (map (instruction_conv \<rho>) (\<pi> @ \<iota> # \<pi>'))) ! 
+        (length (instruction_conv \<rho> \<iota>') + converted_length \<pi> + i) = instruction_conv \<rho> \<iota> ! i" 
       by (simp add: add.assoc del: instr_conv_len)
     thus ?case by simp
   qed
@@ -162,62 +162,54 @@ lemma [simp]: "domain_distinct \<Pi> \<Longrightarrow> lookup \<Pi> s = Some \<p
   program_convert \<Pi> ! (the (build_symbol_table \<Pi> s) + i) = 
     concat (map (instruction_conv (build_symbol_table \<Pi>)) \<pi>) ! i"
   proof -
-    assume D: "domain_distinct \<Pi>"
-       and L: "lookup \<Pi> s = Some \<pi>"
-       and I: "i < converted_length \<pi>"
-    have "\<forall>x. build_symbol_table \<Pi> x = map_option (op + 0) (build_symbol_table \<Pi> x)"
+    assume "domain_distinct \<Pi>"
+       and "lookup \<Pi> s = Some \<pi>"
+       and "i < converted_length \<pi>"
+    moreover have "\<forall>x. build_symbol_table \<Pi> x = map_option (op + 0) (build_symbol_table \<Pi> x)"
       proof
         fix x
         show "build_symbol_table \<Pi> x = map_option (op + 0) (build_symbol_table \<Pi> x)" 
           by (cases "build_symbol_table \<Pi> x") simp_all
       qed
-    with D L I have "program_convert \<Pi> ! (the (build_symbol_table \<Pi> s) - 0 + i) = 
+    ultimately have "program_convert \<Pi> ! (the (build_symbol_table \<Pi> s) - 0 + i) = 
         concat (map (instruction_conv (build_symbol_table \<Pi>)) \<pi>) ! i" 
       by (metis lookup_convert'' program_convert_def)
     thus ?thesis by simp
   qed
 
-lemma lookup_convert: "domain_distinct \<Pi> \<Longrightarrow> pc \<in> get_pc \<Pi> (a # \<pi>) \<Longrightarrow> i < machine_length a \<Longrightarrow>
-    program_convert \<Pi> ! (pc + i) = instruction_conv (build_symbol_table \<Pi>) a ! i"
+lemma lookup_convert: "domain_distinct \<Pi> \<Longrightarrow> pc \<in> get_pc \<Pi> (\<iota> # \<pi>) \<Longrightarrow> i < machine_length \<iota> \<Longrightarrow>
+    program_convert \<Pi> ! (pc + i) = instruction_conv (build_symbol_table \<Pi>) \<iota> ! i"
   proof -
     assume D: "domain_distinct \<Pi>"
-    assume L: "i < machine_length a"
-    assume "pc \<in> get_pc \<Pi> (a # \<pi>)" 
+    assume L: "i < machine_length \<iota>"
+    assume "pc \<in> get_pc \<Pi> (\<iota> # \<pi>)" 
     then obtain s \<pi>' where P: "pc = the (build_symbol_table \<Pi> s) + converted_length \<pi>' \<and> 
-      lookup \<Pi> s = Some (\<pi>' @ a # \<pi>)" by (auto simp add: get_pc_def)
+      lookup \<Pi> s = Some (\<pi>' @ \<iota> # \<pi>)" by (auto simp add: get_pc_def)
     from D L lookup_convert' P show ?thesis by (simp add: add.assoc)
   qed
 
-lemma [simp]: "pc \<in> get_pc \<Pi> (AAssm x # \<pi>) \<Longrightarrow> Suc pc \<in> get_pc \<Pi> \<pi>"
-  proof -
-    assume "pc \<in> get_pc \<Pi> (AAssm x # \<pi>)"
+lemma next_pc: "pc \<in> get_pc \<Pi> (\<iota> # \<pi>) \<Longrightarrow> machine_length \<iota> + pc \<in> get_pc \<Pi> \<pi>"
+  proof (induction \<iota>)
+  case (AAssm x)
     then obtain s \<pi>' where P: "pc = the (build_symbol_table \<Pi> s) + converted_length \<pi>' \<and> 
       lookup \<Pi> s = Some (\<pi>' @ AAssm x # \<pi>)" by (auto simp add: get_pc_def)
     with P have "Suc pc = the (build_symbol_table \<Pi> s) + converted_length (\<pi>' @ [AAssm x])" by simp
-    with P get_pc_def show ?thesis by fastforce
-  qed
-
-lemma [simp]: "pc \<in> get_pc \<Pi> (CAssm dst cmp # \<pi>) \<Longrightarrow> Suc pc \<in> get_pc \<Pi> \<pi>"
-  proof -
-    assume "pc \<in> get_pc \<Pi> (CAssm dst cmp # \<pi>)"
+    with P get_pc_def show ?case by fastforce
+  next case (CAssm dst cmp)
     then obtain s \<pi>' where P: "pc = the (build_symbol_table \<Pi> s) + converted_length \<pi>' \<and> 
       lookup \<Pi> s = Some (\<pi>' @ CAssm dst cmp # \<pi>)" by (auto simp add: get_pc_def)
     with P have "Suc pc = the (build_symbol_table \<Pi> s) + converted_length (\<pi>' @ [CAssm dst cmp])" 
       by simp
-    with P get_pc_def show ?thesis by fastforce
-  qed
-
-lemma [simp]: "pc \<in> get_pc \<Pi> (JAssm jmp s # \<pi>) \<Longrightarrow> Suc (Suc pc) \<in> get_pc \<Pi> \<pi>"
-  proof -
-    assume "pc \<in> get_pc \<Pi> (JAssm jmp s # \<pi>)"
+    with P get_pc_def show ?case by fastforce
+  next case (JAssm jmp s)
     then obtain s' \<pi>' where P: "pc = the (build_symbol_table \<Pi> s') + converted_length \<pi>' \<and> 
       lookup \<Pi> s' = Some (\<pi>' @ JAssm jmp s # \<pi>)" by (auto simp add: get_pc_def)
     with P have "Suc (Suc pc) = 
       the (build_symbol_table \<Pi> s') + converted_length (\<pi>' @ [JAssm jmp s])" by simp
-    with P get_pc_def show ?thesis by fastforce
+    with P get_pc_def show ?case by fastforce
   qed
 
-lemma [simp]: "\<Sigma> \<in> state_convert \<Pi> (\<sigma>, a, d, \<pi>) \<Longrightarrow> \<exists>aa pc. \<Sigma> = (\<sigma>, aa, d, pc) \<and> pc \<in> get_pc \<Pi> \<pi>"
+lemma [simp]: "\<Sigma> \<in> state_convert \<Pi> (\<mu>, a, d, \<pi>) \<Longrightarrow> \<exists>aa pc. \<Sigma> = (\<mu>, aa, d, pc) \<and> pc \<in> get_pc \<Pi> \<pi>"
   by (cases a) auto
 
 lemma eval_assembly_conv [simp]: "domain_distinct \<Pi> \<Longrightarrow> eval_assembly \<Pi> \<Sigma> = Some \<Sigma>\<^sub>1 \<Longrightarrow> 
@@ -226,56 +218,57 @@ lemma eval_assembly_conv [simp]: "domain_distinct \<Pi> \<Longrightarrow> eval_a
   proof (induction \<Pi> \<Sigma> rule: eval_assembly.induct)
   case 1
     thus ?case by simp
-  next case (2 \<Pi> \<sigma> a d x \<pi>)
-    from 2 have S: "\<Sigma>\<^sub>1 = (\<sigma>, Some x, d, \<pi>)" by simp
-    from 2 obtain pc aa where P: "\<Sigma>' = (\<sigma>, aa, d, pc) \<and> pc \<in> get_pc \<Pi> (AAssm x # \<pi>)" by fastforce
-    hence X: "(\<sigma>, x, d, Suc pc) \<in> state_convert \<Pi> (\<sigma>, Some x, d, \<pi>)" by auto
-    from 2 P lookup_convert have "eval_machine (program_convert \<Pi>) (\<sigma>, aa, d, pc) = 
-      Some (\<sigma>, x, d, Suc pc)" by fastforce
+  next case (2 \<Pi> \<mu> a d x \<pi>)
+    from 2 have S: "\<Sigma>\<^sub>1 = (\<mu>, Some x, d, \<pi>)" by simp
+    from 2 obtain pc aa where P: "\<Sigma>' = (\<mu>, aa, d, pc) \<and> pc \<in> get_pc \<Pi> (AAssm x # \<pi>)" by fastforce
+    with next_pc have X: "(\<mu>, x, d, Suc pc) \<in> state_convert \<Pi> (\<mu>, Some x, d, \<pi>)" by fastforce
+    from 2 P lookup_convert have "eval_machine (program_convert \<Pi>) (\<mu>, aa, d, pc) = 
+      Some (\<mu>, x, d, Suc pc)" by fastforce
     with X S P show ?case by fast
-  next case (3 \<Pi> \<sigma> a d dst cmp \<pi>)
-    let ?n = "compute cmp (\<sigma> a) a d"
-    let ?\<sigma> = "if M \<in> dst then \<sigma>(a := ?n) else \<sigma>"
+  next case (3 \<Pi> \<mu> a d dst cmp \<pi>)
+    let ?n = "compute cmp (\<mu> a) a d"
+    let ?\<mu> = "if M \<in> dst then \<mu>(a := ?n) else \<mu>"
     let ?a = "if A \<in> dst then ?n else a"
     let ?d = "if D \<in> dst then ?n else d"
-    from 3 have S: "\<Sigma>\<^sub>1 = (?\<sigma>, Some ?a, ?d, \<pi>)" by (simp add: Let_def)
-    from 3 obtain pc where P: "\<Sigma>' = (\<sigma>, a, d, pc) \<and> pc \<in> get_pc \<Pi> (CAssm dst cmp # \<pi>)" by fastforce
-    hence X: "(?\<sigma>, ?a, ?d, Suc pc) \<in> state_convert \<Pi> (?\<sigma>, Some ?a, ?d, \<pi>)" by auto
-    have "eval_instruction (CInstr dst cmp {}) (\<sigma>, a, d, pc) = (?\<sigma>, ?a, ?d, Suc pc)" 
+    from 3 have S: "\<Sigma>\<^sub>1 = (?\<mu>, Some ?a, ?d, \<pi>)" by (simp add: Let_def)
+    from 3 obtain pc where P: "\<Sigma>' = (\<mu>, a, d, pc) \<and> pc \<in> get_pc \<Pi> (CAssm dst cmp # \<pi>)" by fastforce
+    with next_pc have X: "(?\<mu>, ?a, ?d, Suc pc) \<in> state_convert \<Pi> (?\<mu>, Some ?a, ?d, \<pi>)" by fastforce
+    have "eval_instruction (CInstr dst cmp {}) (\<mu>, a, d, pc) = (?\<mu>, ?a, ?d, Suc pc)" 
       by (simp add: Let_def)
-    with 3 P lookup_convert have "eval_machine (program_convert \<Pi>) (\<sigma>, a, d, pc) = 
-      Some (?\<sigma>, ?a, ?d, Suc pc)" by fastforce
+    with 3 P lookup_convert have "eval_machine (program_convert \<Pi>) (\<mu>, a, d, pc) = 
+      Some (?\<mu>, ?a, ?d, Suc pc)" by fastforce
     with X S P show ?case by fast
   next case 4
     thus ?case by simp
-  next case (5 \<Pi> \<sigma> a d jmp s \<pi>)
-    then obtain pc aa where P: "\<Sigma>' = (\<sigma>, aa, d, pc) \<and> pc \<in> get_pc \<Pi> (JAssm jmp s # \<pi>)" by fastforce
+  next case (5 \<Pi> \<mu> a d jmp s \<pi>)
+    then obtain pc aa where P: "\<Sigma>' = (\<mu>, aa, d, pc) \<and> pc \<in> get_pc \<Pi> (JAssm jmp s # \<pi>)" by fastforce
     let ?s = "get_block_addr (build_symbol_table \<Pi>) s"
-    from 5 P lookup_convert have first_step: "eval_machine (program_convert \<Pi>) (\<sigma>, aa, d, pc) = 
-      Some (\<sigma>, ?s, d, Suc pc)" by fastforce
+    from 5 P lookup_convert have first_step: "eval_machine (program_convert \<Pi>) (\<mu>, aa, d, pc) = 
+      Some (\<mu>, ?s, d, Suc pc)" by fastforce
     show ?case
       proof (cases "should_jump d jmp")
       case True
         thus ?thesis
           proof (cases "lookup \<Pi> s")
           case (Some \<pi>')
-            with 5 True have S: "\<Sigma>\<^sub>1 = (\<sigma>, None, d, \<pi>')" by simp
-            from Some have X: "(\<sigma>, ?s, d, nat ?s) \<in> state_convert \<Pi> (\<sigma>, None, d, \<pi>')" by simp
+            with 5 True have S: "\<Sigma>\<^sub>1 = (\<mu>, None, d, \<pi>')" by simp
+            from Some have X: "(\<mu>, ?s, d, nat ?s) \<in> state_convert \<Pi> (\<mu>, None, d, \<pi>')" by simp
             have "1 < machine_length (JAssm jmp s)" by simp
-            with 5 P lookup_convert True have "eval_machine (program_convert \<Pi>) (\<sigma>, ?s, d, Suc pc) = 
-              Some (\<sigma>, ?s, d, nat ?s)" by fastforce
+            with 5 P lookup_convert True have "eval_machine (program_convert \<Pi>) (\<mu>, ?s, d, Suc pc) = 
+              Some (\<mu>, ?s, d, nat ?s)" by fastforce
             with first_step X P S show ?thesis by fast
           next case None
             with 5 True show ?thesis by simp
           qed
       next case False
-        from 5 False have S: "\<Sigma>\<^sub>1 = (\<sigma>, None, d, \<pi>)" by auto
-        from P have X: "(\<sigma>, ?s, d, Suc (Suc pc)) \<in> state_convert \<Pi> (\<sigma>, None, d, \<pi>)" by auto
-        from False have Y: "eval_instruction (CInstr {} (Reg D) jmp) (\<sigma>, ?s, d, Suc pc) = 
-          (\<sigma>, ?s, d, Suc (Suc pc))" by auto
+        from 5 False have S: "\<Sigma>\<^sub>1 = (\<mu>, None, d, \<pi>)" by auto
+        from P next_pc have X: "(\<mu>, ?s, d, Suc (Suc pc)) \<in> state_convert \<Pi> (\<mu>, None, d, \<pi>)" 
+          by fastforce
+        from False have Y: "eval_instruction (CInstr {} (Reg D) jmp) (\<mu>, ?s, d, Suc pc) = 
+          (\<mu>, ?s, d, Suc (Suc pc))" by auto
         have "1 < machine_length (JAssm jmp s)" by simp
-        with 5 P Y lookup_convert have "eval_machine (program_convert \<Pi>) (\<sigma>, ?s, d, Suc pc) =
-          Some (\<sigma>, ?s, d, Suc (Suc pc))" by fastforce
+        with 5 P Y lookup_convert have "eval_machine (program_convert \<Pi>) (\<mu>, ?s, d, Suc pc) =
+          Some (\<mu>, ?s, d, Suc (Suc pc))" by fastforce
         with first_step X P S show ?thesis by fast
       qed
   qed
