MachineLanguage.thy
@@ -2,25 +2,25 @@ theory MachineLanguage
 imports BasicComputation
 begin
 
-datatype instruction =
+datatype machine_instruction =
   AInstr int
 | CInstr "register set" computation "comparison set"
 
-type_synonym machine_state = "memory \<times> int \<times> int \<times> nat" (* M, A, D, PC *)
+type_synonym machine_state = "memory \<times> int \<times> int \<times> nat" (* \<mu>, a, d, pc *)
 
-fun eval_instruction :: "instruction \<Rightarrow> machine_state \<Rightarrow> machine_state" where
-  "eval_instruction (AInstr x) (\<sigma>, a, d, pc) = (\<sigma>, x, d, Suc pc)"
-| "eval_instruction (CInstr dst cmp jmp) (\<sigma>, a, d, pc) = (
-    let n = compute cmp (\<sigma> a) a d
-    in (if M \<in> dst then \<sigma>(a := n) else \<sigma>, 
+fun eval_instruction :: "machine_instruction \<Rightarrow> machine_state \<Rightarrow> machine_state" where
+  "eval_instruction (AInstr x) (\<mu>, a, d, pc) = (\<mu>, x, d, Suc pc)"
+| "eval_instruction (CInstr dst cmp jmp) (\<mu>, a, d, pc) = (
+    let n = compute cmp (\<mu> a) a d
+    in (if M \<in> dst then \<mu>(a := n) else \<mu>, 
         if A \<in> dst then n else a, 
         if D \<in> dst then n else d, 
         if should_jump n jmp then nat a else Suc pc))"
 
-fun eval_machine :: "instruction list \<Rightarrow> machine_state \<Rightarrow> machine_state option" where
-  "eval_machine \<Pi> (\<sigma>, a, d, pc) = (
+fun eval_machine :: "machine_instruction list \<Rightarrow> machine_state \<Rightarrow> machine_state option" where
+  "eval_machine \<Pi> (\<mu>, a, d, pc) = (
     if pc < length \<Pi> 
-    then Some (eval_instruction (\<Pi> ! pc) (\<sigma>, a, d, pc)) 
+    then Some (eval_instruction (\<Pi> ! pc) (\<mu>, a, d, pc)) 
     else None)"
 
 end
