AssemblyLanguage.thy
@@ -11,24 +11,24 @@ datatype assembly =
 
 type_synonym program = "symbol \<leadsto> assembly list"
 
-type_synonym assembly_state = "memory \<times> int option \<times> int \<times> assembly list" (* M, A, D, PC *)
+type_synonym assembly_state = "memory \<times> int option \<times> int \<times> assembly list" (* \<mu>, a, d, pc *)
 
 fun eval_assembly :: "program \<Rightarrow> assembly_state \<Rightarrow> assembly_state option" where
-  "eval_assembly \<Pi> (\<sigma>, a, d, []) = None"
-| "eval_assembly \<Pi> (\<sigma>, a, d, AAssm x # \<pi>) = Some (\<sigma>, Some x, d, \<pi>)"
-| "eval_assembly \<Pi> (\<sigma>, Some a, d, CAssm dst cmp # \<pi>) = (
-    let n = compute cmp (\<sigma> a) a d
+  "eval_assembly \<Pi> (\<mu>, a, d, []) = None"
+| "eval_assembly \<Pi> (\<mu>, a, d, AAssm x # \<pi>) = Some (\<mu>, Some x, d, \<pi>)"
+| "eval_assembly \<Pi> (\<mu>, Some a, d, CAssm dst cmp # \<pi>) = (
+    let n = compute cmp (\<mu> a) a d
     in Some (
-      if M \<in> dst then \<sigma>(a := n) else \<sigma>, 
+      if M \<in> dst then \<mu>(a := n) else \<mu>, 
       Some (if A \<in> dst then n else a), 
       if D \<in> dst then n else d, 
       \<pi>))"
-| "eval_assembly \<Pi> (\<sigma>, None, d, CAssm dst cmp # \<pi>) = None"
-| "eval_assembly \<Pi> (\<sigma>, a, d, JAssm jmp s # \<pi>) = (
+| "eval_assembly \<Pi> (\<mu>, None, d, CAssm dst cmp # \<pi>) = None"
+| "eval_assembly \<Pi> (\<mu>, a, d, JAssm jmp s # \<pi>) = (
     if should_jump d jmp
     then case lookup \<Pi> s of 
-        Some \<pi>' \<Rightarrow> Some (\<sigma>, None, d, \<pi>')
+        Some \<pi>' \<Rightarrow> Some (\<mu>, None, d, \<pi>')
       | None \<Rightarrow> None
-    else Some (\<sigma>, None, d, \<pi>))"
+    else Some (\<mu>, None, d, \<pi>))"
 
 end
